lean/src/internal/Ant/implies.lean
@@ -1,12 +1,8 @@
 import tactic
 import data.finset
-import ...definitions
 import ..internal_definitions
 import .leaves
-import ..tactics
-import ..utils
 import .map
-import ..U
 
 variable [GuardModule]
 open GuardModule
@@ -15,18 +11,9 @@ open GuardModule
 begin
     induction h1 generalizing c;
     cases h2,
-    {
-        refine Ant.implies.leaf _,
-        tauto,
-    }, {
-        refine Ant.implies.branch _ _,
-        tauto,
-        tauto,
-    }, {
-        refine Ant.implies.diverge _ _,
-        tauto,
-        tauto,
-    },
+    { refine Ant.implies.leaf _; tauto, },
+    { refine Ant.implies.branch _ _; tauto, },
+    { refine Ant.implies.diverge _ _; tauto, },
 end
 
 @[refl] lemma Ant.implies_refl (a : Ant bool) : a ⟶ a :=
@@ -34,10 +21,7 @@ by induction a; simp [Ant.implies.leaf, Ant.implies.branch, Ant.implies.diverge,
 
 lemma Ant.implies_equal_structure { a b: Ant bool } (h: a ⟶ b):
     a.map (λ x, false) = b.map (λ x, false) :=
-begin
-    induction h;
-    simp [Ant.map, *],
-end
+by induction h; simp [Ant.map, *]
 
 lemma Ant.implies_same_leaves { a b: Ant bool } (h: a ⟶ b): a.leaves = b.leaves :=
 begin
