lean/src/internal/Ant/map.lean
@@ -1,9 +1,7 @@
 import tactic
-import data.finset
 import ...definitions
 import ..internal_definitions
 import ..utils
-import ..tactics
 
 variable [GuardModule]
 open GuardModule
