lean/src/internal/result.lean
@@ -8,28 +8,16 @@ open GuardModule
 
 @[simp]
 lemma Result.is_match_tt_neq_no_match (r: Result): r.is_match = tt ↔ r ≠ Result.no_match :=
-begin
-    cases r;
-    simp [Result.is_match],
-end
+by cases r; simp [Result.is_match]
 
 @[simp]
 lemma Result.is_match_ff_neq_no_match (r: Result): r.is_match = ff ↔ r = Result.no_match :=
-begin
-    cases r;
-    simp [Result.is_match],
-end
+by cases r; simp [Result.is_match]
 
 @[simp]
 lemma Result.is_match_neq_no_match (r: Result): r.is_match ↔ r ≠ Result.no_match :=
-begin
-    cases r;
-    simp [Result.is_match],
-end
+by cases r; simp [Result.is_match]
 
 @[simp]
 lemma Result.not_is_match_eq_no_match (r: Result): !r.is_match ↔ r = Result.no_match :=
-begin
-    cases r;
-    simp [Result.is_match],
-end
+by cases r; simp [Result.is_match]
